adder: adequacy

theories/examples/counter_adequacy.v
@@ -7,7 +7,7 @@ From cap_machine Require Import
      stdpp_extra iris_extra
      rules logrel fundamental.
 From cap_machine.examples Require Import
-     macros malloc counter_preamble disjoint_regions_tactics.
+     macros malloc counter_preamble disjoint_regions_tactics mkregion_helpers.
 
 Instance DisjointList_list_Addr : DisjointList (list Addr).
 Proof. exact (@disjoint_list_default _ _ app []). Defined.
@@ -93,9 +93,6 @@ Class memory_layout `{MachineParameters} := {
        ];
 }.
 
-Definition mkregion (r_start r_end: Addr) (contents: list Word): gmap Addr Word :=
-  list_to_map (zip (region_addrs r_start r_end) contents).
-
 Definition offset_to_awkward `{memory_layout} : Z :=
   (* in this setup, the body of the counter comes just after the code
      of the preamble *)
@@ -172,99 +169,6 @@ Section Adequacy.
   Context {reg_preg: gen_heapPreG RegName Word Σ}.
   Context {na_invg: na_invG Σ}.
   Context `{MP: MachineParameters}.
-
-  
-  Lemma dom_mkregion_incl a e l:
-    dom (gset Addr) (mkregion a e l) ⊆ list_to_set (region_addrs a e).
-  Proof.
-    rewrite /mkregion. generalize (region_addrs a e). induction l.
-    { intros. rewrite zip_with_nil_r /=. rewrite dom_empty_L. apply empty_subseteq. }
-    { intros ll. destruct ll as [| x ll].
-      - cbn. rewrite dom_empty_L. done.
-      - cbn [list_to_set zip zip_with list_to_map foldr fst snd]. rewrite dom_insert_L.
-        set_solver. }
-  Qed.
-
-  Lemma dom_mkregion_incl_rev a e l:
-    (a + length l = Some e)%a →
-    list_to_set (region_addrs a e) ⊆ dom (gset Addr) (mkregion a e l).
-  Proof.
-    rewrite /mkregion. intros Hl.
-    assert (length (region_addrs a e) = length l) as Hl'.
-    { rewrite region_addrs_length /region_size. solve_addr. }
-    clear Hl. revert Hl'. generalize (region_addrs a e). induction l.
-    { intros. rewrite zip_with_nil_r /=. rewrite dom_empty_L.
-      destruct l; [| inversion Hl']. cbn. apply empty_subseteq. }
-    { intros ll Hll. destruct ll as [| x ll]; [by inversion Hll|].
-      cbn [list_to_set zip zip_with list_to_map foldr fst snd].
-      rewrite dom_insert_L. cbn in Hll. apply Nat.succ_inj in Hll.
-      specialize (IHl ll Hll). set_solver. }
-  Qed.
-
-  Lemma dom_mkregion_eq a e l:
-    (a + length l = Some e)%a →
-    dom (gset Addr) (mkregion a e l) = list_to_set (region_addrs a e).
-  Proof.
-    intros Hlen. apply (anti_symm _).
-    - apply dom_mkregion_incl.
-    - by apply dom_mkregion_incl_rev.
-  Qed.
-
-  Lemma in_dom_mkregion a e l k:
-    k ∈ dom (gset Addr) (mkregion a e l) →
-    k ∈ region_addrs a e.
-  Proof.
-    intros H.
-    pose proof (dom_mkregion_incl a e l) as HH.
-    rewrite elem_of_subseteq in HH |- * => HH.
-    specialize (HH _ H). eapply elem_of_list_to_set; eauto.
-  Qed.
-
-  Lemma in_dom_mkregion' a e l k:
-    (a + length l = Some e)%a →
-    k ∈ region_addrs a e →
-    k ∈ dom (gset Addr) (mkregion a e l).
-  Proof.
-    intros. rewrite dom_mkregion_eq // elem_of_list_to_set //.
-  Qed.
-
-  Ltac disjoint_map_to_list :=
-    rewrite (@map_disjoint_dom _ _ (gset Addr)) ?dom_union_L;
-    eapply disjoint_mono_l;
-    rewrite ?dom_list_to_map_singleton;
-    repeat (
-      try lazymatch goal with
-          | |- _ ∪ _ ⊆ _ =>
-            etransitivity; [ eapply union_mono_l | eapply union_mono_r ]
-          end;
-      [ first [ apply dom_mkregion_incl | reflexivity ] |..]
-    );
-    try match goal with |- _ ## dom _ (mkregion _ _ _) =>
-      eapply disjoint_mono_r; [ apply dom_mkregion_incl |] end;
-    rewrite -?list_to_set_app_L ?dom_list_to_map_singleton;
-    apply list_to_set_disj.
-
-  Lemma mkregion_sepM_to_sepL2 (a e: Addr) l (φ: Addr → Word → iProp Σ) :
-    (a + length l)%a = Some e →
-    ([∗ map] k↦v ∈ mkregion a e l, φ k v) -∗ ([∗ list] k;v ∈ (region_addrs a e); l, φ k v).
-  Proof.
-    rewrite /mkregion. revert a e. induction l as [| x l].
-    { cbn. intros. rewrite zip_with_nil_r /=. assert (a = e) as -> by solve_addr.
-      rewrite /region_addrs region_size_0. 2: solve_addr. cbn. eauto. }
-    { cbn. intros a e Hlen. rewrite region_addrs_cons. 2: solve_addr.
-      cbn. iIntros "H". iDestruct (big_sepM_insert with "H") as "[? H]".
-      { rewrite -not_elem_of_list_to_map /=.
-        intros [ [? ?] [-> [? ?]%elem_of_zip_l%elem_of_region_addrs] ]%elem_of_list_fmap.
-        solve_addr. }
-      iFrame. iApply (IHl with "H"). solve_addr. }
-  Qed.
-
-  Lemma mkregion_prepare `{memG Σ} (a e: Addr) l :
-    (a + length l)%a = Some e →
-    ([∗ map] k↦v ∈ mkregion a e l, k ↦ₐ v) ==∗ ([∗ list] k;v ∈ (region_addrs a e); l, k ↦ₐ v).
-  Proof.
-    iIntros (?) "H". iDestruct (mkregion_sepM_to_sepL2 with "H") as "H"; auto.
-  Qed.
 
   Definition flagN : namespace := nroot .@ "awk" .@ "fail_flag".
   Definition mallocN : namespace := nroot .@ "awk" .@ "malloc".
