theories/examples/adder_adequacy.v
@@ -1,0 +1,259 @@
+From iris.algebra Require Import auth agree excl gmap frac.
+From iris.proofmode Require Import tactics.
+From iris.base_logic Require Import invariants.
+From iris.program_logic Require Import adequacy.
+Require Import Eqdep_dec.
+From cap_machine Require Import
+     stdpp_extra iris_extra
+     rules logrel fundamental.
+From cap_machine.examples Require Import
+     macros malloc adder disjoint_regions_tactics mkregion_helpers.
+
+Instance DisjointList_list_Addr : DisjointList (list Addr).
+Proof. exact (@disjoint_list_default _ _ app []). Defined.
+
+Class memory_layout `{MachineParameters} := {
+  (* Code of g and f *)
+  g_start : Addr;
+  f_start : Addr;
+  f_end : Addr;
+
+  (* Memory cell for x *)
+  x : Addr;
+  x' : Addr; (* x' = x+1 *)
+
+  (* Memory for the activation record *)
+  act_start : Addr;
+  act_end : Addr;
+
+  (* adversary code *)
+  adv_start : Addr;
+  adv_end : Addr;
+
+  g_size :
+    (g_start + adder_g_instrs_length)%a = Some f_start;
+  f_size :
+    (f_start + adder_f_instrs_length)%a = Some f_end;
+
+  act_size :
+    (act_start + 8)%a = Some act_end;
+
+  x_size :
+    (x + 1)%a = Some x';
+
+  (* disjointness of all the regions above *)
+  regions_disjoint :
+    ## [
+        region_addrs adv_start adv_end;
+        region_addrs act_start act_end;
+        [x];
+        region_addrs f_start f_end;
+        region_addrs g_start f_start
+       ]
+}.
+
+Definition mk_initial_memory `{memory_layout} (adv_val act_val : list Word) : gmap Addr Word :=
+    mkregion g_start f_start (adder_g_instrs f_start f_end)
+  ∪ mkregion f_start f_end adder_f_instrs
+  ∪ list_to_map [(x, inl 0%Z)] (* x: initially set to 0 (could be any positive number) *)
+  ∪ mkregion act_start act_end act_val (* the activation region can hold arbitrary words *)
+  ∪ mkregion adv_start adv_end adv_val
+    (* adversarial code: any code or data, but no capabilities
+       (see condition below) *)
+.
+
+Definition is_initial_memory `{memory_layout} (m: gmap Addr Word) :=
+  ∃ (adv_val act_val: list Word),
+    m = mk_initial_memory adv_val act_val
+  (* The adversarial region in memory must only contain instructions, no
+     capabilities (it can thus only access the capability [g] passes it
+     through the registers, including a capability to the adversarial region
+     (so the adversarial code *CAN* access (RWX) its own memory)
+  *)
+  ∧ Forall (λ w, is_cap w = false) adv_val
+  ∧ length act_val = 8
+  ∧ (adv_start + length adv_val)%a = Some adv_end.
+
+Definition is_initial_registers `{memory_layout} (reg: gmap RegName Word) :=
+  reg !! PC = Some (inr (RX, g_start, f_end, g_start)) ∧
+  reg !! r_t0 = Some (inr (RWX, adv_start, adv_end, adv_start)) ∧
+  reg !! r_t1 = Some (inr (RWX, act_start, act_end, act_start)) ∧
+  reg !! r_t3 = Some (inr (RW, x, x', x)) ∧
+  (∀ (r: RegName), r ∉ ({[ PC; r_t0; r_t1; r_t3 ]} : gset RegName) →
+     ∃ (w:Word), reg !! r = Some w ∧ is_cap w = false).
+
+Lemma initial_registers_full_map `{MachineParameters, memory_layout} reg :
+  is_initial_registers reg →
+  (∀ r, is_Some (reg !! r)).
+Proof.
+  intros (HPC & Hr0 & Hr1 & Hr3 & Hothers) r.
+  destruct (decide (r = PC)) as [->|]. by eauto.
+  destruct (decide (r = r_t0)) as [->|]. by eauto.
+  destruct (decide (r = r_t1)) as [->|]. by eauto.
+  destruct (decide (r = r_t3)) as [->|]. by eauto.
+  destruct (Hothers r) as (w & ? & ?); [| eauto]. set_solver.
+Qed.
+
+Section Adequacy.
+  Context (Σ: gFunctors).
+  Context {inv_preg: invPreG Σ}.
+  Context {mem_preg: gen_heapPreG Addr Word Σ}.
+  Context {reg_preg: gen_heapPreG RegName Word Σ}.
+  Context {na_invg: na_invG Σ}.
+  Context `{MP: MachineParameters}.
+
+  Definition invN : namespace := nroot .@ "adder" .@ "inv".
+
+  Lemma adder_adequacy' {ML:memory_layout} (m m': Mem) (reg reg': Reg) (es: list cap_lang.expr):
+    is_initial_memory m →
+    is_initial_registers reg →
+    rtc erased_step ([Seq (Instr Executable)], (reg, m)) (es, (reg', m')) →
+    ∃ (n: Z), m' !! x = Some (inl n) ∧ (n >= 0)%Z.
+  Proof.
+    intros Hm Hreg Hstep.
+    pose proof (@wp_invariance Σ cap_lang _ NotStuck) as WPI. cbn in WPI.
+    pose (fun (c:ExecConf) => ∃ n, c.2 !! x = Some (inl n) ∧ (n >= 0)%Z) as state_is_good.
+    specialize (WPI (Seq (Instr Executable)) (reg, m) es (reg', m') (state_is_good (reg', m'))).
+    eapply WPI. 2: assumption. intros Hinv κs. clear WPI.
+
+    unfold is_initial_memory in Hm.
+    destruct Hm as (adv_val & act_val & Hm & Hadv_val & act_len & adv_size).
+    iMod (gen_heap_init (∅:Mem)) as (mem_heapg) "Hmem_ctx".
+    iMod (gen_heap_init (∅:Reg)) as (reg_heapg) "Hreg_ctx".
+    iMod (@na_alloc Σ na_invg) as (logrel_nais) "Hna".
+
+    pose memg := MemG Σ Hinv mem_heapg.
+    pose regg := RegG Σ Hinv reg_heapg.
+    pose logrel_na_invs := Build_logrel_na_invs _ na_invg logrel_nais.
+
+    pose proof (
+      @adder_full_spec Σ memg regg logrel_na_invs MP invN f_start f_end
+    ) as Spec.
+
+    iMod (gen_heap_alloc_gen _ reg with "Hreg_ctx") as "(Hreg_ctx & Hreg & _)".
+      by apply map_disjoint_empty_r. rewrite right_id_L.
+    iMod (gen_heap_alloc_gen _ m with "Hmem_ctx") as "(Hmem_ctx & Hmem & _)".
+      by apply map_disjoint_empty_r. rewrite right_id_L.
+
+    (* Extract points-to for the various regions in memory *)
+
+    pose proof regions_disjoint as Hdisjoint.
+    rewrite {2}Hm.
+    rewrite disjoint_list_cons in Hdisjoint |- *. intros (Hdisj_adv & Hdisjoint).
+    iDestruct (big_sepM_union with "Hmem") as "[Hmem Hadv]".
+    { disjoint_map_to_list. set_solver +Hdisj_adv. }
+    rewrite disjoint_list_cons in Hdisjoint |- *. intros (Hdisj_act & Hdisjoint).
+    iDestruct (big_sepM_union with "Hmem") as "[Hmem Hact]".
+    { disjoint_map_to_list. set_solver +Hdisj_act. }
+    rewrite disjoint_list_cons in Hdisjoint |- *. intros (Hdisj_x & Hdisjoint).
+    iDestruct (big_sepM_union with "Hmem") as "[Hmem Hx]".
+    { disjoint_map_to_list. set_solver +Hdisj_x. }
+    iDestruct (big_sepM_insert with "Hx") as "[Hx _]". by apply lookup_empty. cbn [fst snd].
+    rewrite disjoint_list_cons in Hdisjoint |- *. intros (Hdisj_f & Hdisjoint).
+    iDestruct (big_sepM_union with "Hmem") as "[Hg Hf]".
+    { disjoint_map_to_list. set_solver +Hdisj_f. }
+    rewrite disjoint_list_cons in Hdisjoint |- *. intros (Hdisj_g & _).
+    clear Hdisj_adv Hdisj_act Hdisj_x Hdisj_f Hdisj_g.
+
+    (* Massage points-to into sepL2s with permission-pointsto *)
+
+    iDestruct (mkregion_prepare with "Hf") as ">Hf". by apply f_size.
+    iDestruct (mkregion_prepare with "Hg") as ">Hg". by apply g_size.
+    iDestruct (mkregion_prepare with "Hact") as ">Hact".
+      rewrite act_len; by apply act_size.
+    iDestruct (mkregion_prepare with "Hadv") as ">Hadv". by apply adv_size.
+
+    (* Allocate the invariant about x *)
+
+    iMod (inv_alloc invN ⊤ (∃ n, x ↦ₐ inl n ∗ ⌜(0 ≤ n)%Z⌝)%I with "[Hx]") as "#Hinv".
+    { iNext. eauto. }
+
+    (* Establish that the adversary region is valid *)
+
+    iMod (region_inv_alloc with "[Hadv]") as "Hadv".
+    { iApply (big_sepL2_mono with "Hadv").
+      intros k v1 v2 Hv1 Hv2. cbn. iIntros. iFrame.
+      pose proof (Forall_lookup_1 _ _ _ _ Hadv_val Hv2) as Hncap.
+      destruct v2; [| by inversion Hncap].
+      rewrite fixpoint_interp1_eq /=. done. }
+    iDestruct "Hadv" as "#Hadv".
+
+    (* Prepare the registers *)
+
+    unfold is_initial_registers in Hreg.
+    destruct Hreg as (HPC & Hr0 & Hr1 & Hr3 & Hrothers).
+    iDestruct (big_sepM_delete _ _ PC with "Hreg") as "[HPC Hreg]"; eauto.
+    iDestruct (big_sepM_delete _ _ r_t0 with "Hreg") as "[Hr0 Hreg]".
+    by rewrite lookup_delete_ne //.
+    iDestruct (big_sepM_delete _ _ r_t1 with "Hreg") as "[Hr1 Hreg]".
+    by rewrite !lookup_delete_ne //.
+    iDestruct (big_sepM_delete _ _ r_t3 with "Hreg") as "[Hr3 Hreg]".
+    by rewrite !lookup_delete_ne //.
+    destruct (Hrothers r_t2) as [r2v [Hr2v Hr2V] ]. set_solver+.
+    iDestruct (big_sepM_delete _ _ r_t2 with "Hreg") as "[Hr2 Hreg]".
+    by rewrite !lookup_delete_ne //.
+
+    match goal with |- context [([∗ map] _↦_ ∈ ?r, _)%I] => set rmap := r end.
+    iAssert ([∗ map] r↦w ∈ rmap, (r ↦ᵣ w ∗ interp w))%I with "[Hreg]" as "Hreg".
+    { iApply (big_sepM_mono with "Hreg"). intros r w Hr. cbn.
+      iIntros "?". iFrame. rewrite fixpoint_interp1_eq.
+      assert (HH: r ∈ dom (gset RegName) rmap). by apply elem_of_gmap_dom; eauto.
+      rewrite /rmap !dom_delete_L in HH.
+      destruct (Hrothers r) as [w' [? Hncap] ].
+      { subst rmap. set_solver+ HH. }
+      subst rmap. repeat (rewrite lookup_delete_ne in Hr; [|set_solver+ HH]).
+      simplify_eq. destruct w'; [|by inversion Hncap]. eauto. }
+
+    assert (∀ r, is_Some (reg !! r)) as Hreg_full.
+    { intros r.
+      destruct (decide (r = PC)); subst; [by eauto|].
+      destruct (decide (r = r_t0)); subst; [by eauto|].
+      destruct (decide (r = r_t1)); subst; [by eauto|].
+      destruct (decide (r = r_t3)); subst; [by eauto|].
+      destruct (Hrothers r) as [? [? ?] ]; eauto. set_solver. }
+
+    (* Use the resources to instantiate the spec and obtain a WP *)
+
+    iPoseProof (Spec with "[$HPC $Hr0 $Hr1 $Hr2 $Hr3 $Hreg $Hna $Hf $Hg $Hact]")
+      as "SpecWP".
+    { apply contiguous_between_region_addrs. generalize g_size; clear; solve_addr. }
+    { apply contiguous_between_region_addrs. generalize f_size; clear; solve_addr. }
+    { apply x_size. }
+    { apply act_size. }
+    { generalize f_size; clear; solve_addr. }
+    { subst rmap. rewrite !dom_delete_L regmap_full_dom. set_solver+.
+      apply Hreg_full. }
+    { iFrame "Hinv". rewrite fixpoint_interp1_eq /=.
+      iDestruct (big_sepL2_to_big_sepL_l with "Hadv") as "Hadv'".
+      { rewrite region_addrs_length /region_size.
+        generalize adv_size. clear; solve_addr. }
+      iApply (big_sepL_mono with "Hadv'"). iIntros (? ? ?) "Hw". cbn.
+      iExists _. iFrame "Hw". iSplit; eauto. }
+
+    (* We get a WP; conclude using the rest of the Iris adequacy theorem *)
+
+    iModIntro.
+    (* Must match the state_interp of [memG_irisG] in rules_base.v *)
+    iExists (fun σ κs _ => ((gen_heap_ctx σ.1) ∗ (gen_heap_ctx σ.2)))%I.
+    iExists (fun _ => True)%I. cbn. iFrame.
+    iIntros "[Hreg' Hmem']". iExists (⊤ ∖ ↑invN).
+    iInv invN as ">Hx" "_".
+    iDestruct "Hx" as (n) "[Hx %]".
+    iDestruct (gen_heap_valid with "Hmem' Hx") as %Hm'_x.
+    iModIntro. iPureIntro. rewrite /state_is_good //.
+    exists n. cbn. split; eauto. lia.
+  Qed.
+
+End Adequacy.
+
+Theorem adder_adequacy `{MachineParameters} `{memory_layout}
+        (m m': Mem) (reg reg': Reg) (es: list cap_lang.expr):
+  is_initial_memory m →
+  is_initial_registers reg →
+  rtc erased_step ([Seq (Instr Executable)], (reg, m)) (es, (reg', m')) →
+  ∃ (n: Z), m' !! x = Some (inl n) ∧ (n >= 0)%Z.
+Proof.
+  set (Σ := #[invΣ; gen_heapΣ Addr Word; gen_heapΣ RegName Word;
+              na_invΣ]).
+  eapply (@adder_adequacy' Σ); typeclasses eauto.
+Qed.
